total/streams.v
@@ -1,0 +1,200 @@
+Require Import ssreflect ssrfun ssrbool eqtype ssrnat seq.
+Require Import Utf8.
+
+Set Implicit Arguments.
+Unset Strict Implicit.
+Unset Printing Implicit Defensive.
+
+Section Streams.
+Variable A : Type.
+
+CoInductive Stream :=
+  | Nil : Stream
+  | Cons : A -> Stream -> Stream.
+
+Definition Stream_decompose (s : Stream) : Stream :=
+  match s with
+    | Nil => Nil
+    | Cons h t => Cons h t
+  end.
+
+Lemma Stream_decompose_lemma s : s = Stream_decompose s.
+Proof.
+by case: s.
+Qed.
+
+(*Lemma Stream_unfold x :
+  x = match x with
+        | Nil => Nil
+        | Cons a s => Cons a s
+      end.
+Proof. by case: x. Qed.*)
+
+Lemma not_Nil_Cons s :
+  ~ s = Nil -> exists h t, s = Cons h t.
+Proof.
+case: s => [// |]; by eauto.
+Qed.
+
+Fixpoint seqToStream (s : seq A) : Stream :=
+  match s with
+    | [::] => Nil
+    | h :: t => Cons h (seqToStream t)
+  end.
+
+Fixpoint firstN n (s : Stream) : seq A :=
+  match n with
+    | 0 => [::]
+    | n.+1 =>
+        match s with
+          | Nil => [::]
+          | Cons h t => h :: firstN n t
+        end
+  end.
+
+Fixpoint catSeqStream (s1 : seq A) (s2 : Stream) : Stream :=
+  match s1 with
+    | [::] => s2
+    | h :: t => Cons h (catSeqStream t s2)
+  end.
+
+Lemma catSeqStream_cat s1 s2 s3 :
+  catSeqStream s1 (catSeqStream s2 s3) =
+  catSeqStream (s1 ++ s2) s3.
+Proof.
+elim: s1 => [| h t IH] //=.
+by rewrite IH.
+Qed.
+
+Lemma catSeqStream_Nil s :
+  catSeqStream s Nil = seqToStream s.
+Proof.
+elim: s => [| h t IH] //=.
+by rewrite IH.
+Qed.
+
+Lemma catSeqStream_firstN s p r :
+  s = catSeqStream p r -> exists n, p = firstN n s.
+Proof.
+move: s.
+elim: p => [| h t IH].
+- rewrite /=. by move => s _; exists 0.
+- move => s e.
+  rewrite /= in e.
+  elim: (IH _ Logic.eq_refl) => n Hn.
+  exists n.+1.
+  by rewrite e [in X in X = _]Hn.
+Qed.
+
+(*CoFixpoint catStream (s1 s2 : Stream) : Stream :=
+  match s1 with
+    | Nil => s2
+    | Cons h t => Cons h (catStream t s2)
+  end.
+
+Lemma catStream_nil (s : Stream) :
+  catSeqStream [::] s = s.
+by [].
+Qed.
+
+Definition catSeqStream_bis (s1 : seq A) (s2 : Stream)
+  := catStream (seqToStream s1) s2.*)
+
+CoFixpoint funToStream_from n (f : nat -> A) : Stream
+  := Cons (f n) (funToStream_from n.+1 f).
+
+Definition funToStream f := funToStream_from 0 f.
+
+Inductive Finite : Stream -> Prop :=
+  | Nil_fin : Finite Nil
+  | Cons_fin : forall a s, Finite s -> Finite (Cons a s).
+
+CoInductive Infinite : Stream -> Prop :=
+  | Cons_inf : forall a s, Infinite s -> Infinite (Cons a s).
+
+Lemma seq_Finite s : Finite (seqToStream s).
+Proof.
+elim: s => [| h t IH] //=; by constructor.
+Qed.
+
+Lemma catSeqStream_Finite s1 s2 :
+  Finite s2 -> Finite (catSeqStream s1 s2).
+Proof.
+elim: s1 => [| h t IH] //=.
+move => H. by constructor; auto.
+Qed.
+
+Lemma Infinite_elim s :
+  Infinite s -> exists a t, s = Cons a t /\ Infinite t.
+Proof.
+case; by eauto.
+Qed.
+
+Lemma Infinite_not_Nil s : Infinite s -> ~ s = Nil.
+Proof.
+move => Hinf.
+elim: (Infinite_elim Hinf) => h [t [? _]].
+by subst s.
+Qed.
+
+Lemma catSeqStream_Infinite_1 l s :
+  Infinite s -> Infinite (catSeqStream l s).
+Proof.  
+elim: l => [| a h IH]; by intuition.
+Qed.
+
+Lemma catSeqStream_Infinite_2 l s :
+  Infinite (catSeqStream l s) -> Infinite s.
+Proof.
+elim: l => [| a h IH] //=.
+move => H. by inversion H; intuition.
+Qed.
+
+Lemma funToStream_from_unfold n f :
+  funToStream_from n f = Cons (f n) (funToStream_from n.+1 f).
+Proof.
+by rewrite [X in X = _] Stream_decompose_lemma.
+Qed.
+
+Lemma funToStream_from_Infinite f :
+  forall n, Infinite (funToStream_from n f).
+Proof.
+cofix H.
+move => n.
+rewrite funToStream_from_unfold.
+constructor.
+by apply: H.
+Qed.
+
+Lemma funToStream_Infinite f : Infinite (funToStream f).
+Proof.
+by apply: funToStream_from_Infinite.
+Qed.
+
+Lemma Nil_not_Infinite : ~ Infinite Nil.
+Proof.
+move => H. by inversion H.
+Qed.
+Hint Resolve Nil_not_Infinite.
+
+Lemma Finite_not_Infinite s :
+  Finite s -> ~ Infinite s.
+Proof.
+move => H. elim: H => //.
+move => h t Hf Hi Hicons.
+case: Hi. by inversion Hicons.
+Qed.
+
+Lemma not_Finite_Infinite s :
+  ~ Finite s -> Infinite s.
+Proof.
+move: s. cofix H. case.
+- by have Habs : Finite Nil by constructor.
+- move => h t Hcons.
+  constructor.
+  apply: H => H. elim: Hcons. by constructor.
+Qed.
+
+End Streams.
+
+Arguments Nil [A] : default implicits.
